WIP

CpsatScheduler/UnitScale.lean
@@ -1,5 +1,7 @@
 import CpsatScheduler.Defs
 
+import Mathlib.Data.Finset.Sort
+
 namespace CpsatScheduler
 
 instance : DecidableLE UnitScale :=
@@ -25,6 +27,57 @@ def UnitScale.exactRatio (u v : UnitScale) (_hv : v.val ∣ u.val) :
 
 instance : Coe UnitScale CpsatSolver.Int64 where
   coe v := Subtype.mk (v.val : ℤ) v.nonoverflow
+
+private def sortPred (a b : UnitScale) : Prop :=
+  a.val ≤ b.val
+
+instance : Std.Antisymm sortPred where
+  antisymm a b rab rba : a = b := by
+    dsimp [sortPred] at rab
+    dsimp [sortPred] at rba
+    apply LE.le.eq_or_lt at rab
+    apply LE.le.eq_or_lt at rba
+    cases a
+    cases b
+    simp only [UnitScale.mkRaw.injEq]
+    simp only at rab
+    simp only at rba
+    cases rab with
+    | inl heq =>
+      cases rba with
+      | inl _ =>
+        cases heq
+        rfl
+      | inr _ =>
+        by_contra
+        contradiction
+    | inr a_lt_b =>
+      cases rba with
+      | inl heq =>
+        cases heq
+        rfl
+      | inr b_lt_a =>
+        apply LT.lt.asymm at a_lt_b
+        contradiction
+
+instance : DecidableRel sortPred :=
+  fun a b => inferInstanceAs (Decidable (a.val ≤ b.val))
+
+instance : IsTrans UnitScale sortPred where
+  trans _ _ _ rab rbc := LE.le.trans rab rbc
+
+instance : Std.Total sortPred where
+  total a b := le_total a.val b.val
+
+def UnitScale.sort (s : Finset UnitScale) : List UnitScale :=
+  Finset.sort s sortPred
+
+theorem UnitScale.mem_sort {us : Finset UnitScale}
+  (u : UnitScale) (u_in_list : u ∈ UnitScale.sort us) :
+    u ∈ us := by
+      dsimp [sort] at u_in_list
+      apply (us.mem_sort sortPred).mp at u_in_list
+      exact u_in_list
 
 end CpsatScheduler
 
